Typing.v
@@ -28,61 +28,60 @@ Proof.
   introv Ht Hv.
   apply validated_typing in Ht.
   remember (E & G) as EG.
-  generalize dependent E.
   generalize dependent G.
-  generalize dependent F.
   induction Ht; introv Heq Hv; subst;
     eauto using valid_instance_weakening, binds_weakening,
-                kinding_weakening, subtype_weakening
+                kinding_weakening, subtype_weakening,
+                type_equal_weakening
           with valid_env_regular.    
-  - apply typing_abs with (L := L \u dom E0 \u dom F \u dom G);
+  - apply typing_abs with (L := L \u dom E \u dom F \u dom G);
       auto using kinding_weakening.
     intros x Hn.
-    assert (valid_env (E0 & F & G & x ~: sch_empty T1))
+    assert (valid_env (E & F & G & x ~: sch_empty T1))
       as He by auto using valid_env_type_weakening.
     rewrite <- concat_assoc.
     rewrite <- concat_assoc in He.
     auto using concat_assoc.
   - apply typing_let
-      with (M := M) (L := L \u dom E0 \u dom F \u dom G).
+      with (M := M) (L := L \u dom E \u dom F \u dom G).
     + intros Xs Hl.
-      assert (valid_env (E0 & F & G & Xs ~::* M))
+      assert (valid_env (E & F & G & Xs ~::* M))
         as He by auto using valid_env_kinds_weakening.
       rewrite <- concat_assoc.
       rewrite <- concat_assoc in He.
       auto using concat_assoc.
     + intros x Hl.
-      assert (valid_env (E0 & F & G & x ~: M))
+      assert (valid_env (E & F & G & x ~: M))
         as He by auto using valid_env_type_weakening.
       rewrite <- concat_assoc.
       rewrite <- concat_assoc in He.
       auto using concat_assoc.
   - apply typing_match
-      with (L := L \u dom E0 \u dom F \u dom G)
+      with (L := L \u dom E \u dom F \u dom G)
            (T1 := T1) (T2 := T2) (T3 := T3) (T4 := T4)
            (T5 := T5) (T6 := T6) (T7 := T7);
       auto using kinding_weakening, subtype_weakening.
     + intros x Hn.
       assert
-        (valid_env (E0 & F & G & x ~: sch_empty (typ_variant T3)))
+        (valid_env (E & F & G & x ~: sch_empty (typ_variant T3)))
         as He by auto using valid_env_type_weakening.
       rewrite <- concat_assoc.
       rewrite <- concat_assoc in He.
       auto using concat_assoc.
     + intros y Hn.
       assert
-        (valid_env (E0 & F & G & y ~: sch_empty (typ_variant T5)))
+        (valid_env (E & F & G & y ~: sch_empty (typ_variant T5)))
         as He by auto using valid_env_type_weakening.
       rewrite <- concat_assoc.
       rewrite <- concat_assoc in He.
       auto using concat_assoc.
   - apply typing_destruct
-      with (L := L \u dom E0 \u dom F \u dom G)
+      with (L := L \u dom E \u dom F \u dom G)
            (T1 := T1) (T2 := T2) (T3 := T3);
       auto using kinding_weakening, subtype_weakening.
     intros x Hn.
     assert
-      (valid_env (E0 & F & G & x ~: sch_empty T3))
+      (valid_env (E & F & G & x ~: sch_empty T3))
       as He by auto using valid_env_type_weakening.
     rewrite <- concat_assoc.
     rewrite <- concat_assoc in He.
@@ -106,16 +105,18 @@ Lemma typing_typ_subst : forall E F X K S t T,
 Proof.
   introv Ht Hk.
   remember (E & X ~:: K & F) as EXF.
-  generalize dependent E.
   generalize dependent F.
-  induction Ht; introv Heq Hk; subst; eauto.
+  induction Ht; introv Heq; subst; eauto.
   - apply typing_var
         with (M := sch_subst X S M)
              (Us := (List.map (typ_subst X S) Us));
       eauto using valid_env_typ_subst, valid_instance_typ_subst,
                   sch_subst_instance, binds_typ_typ_subst
             with kinding_regular.
-  - apply typing_abs with (L := L \u \{X} \u dom E0 \u dom F).
+    replace knd_type with (knd_subst X S knd_type) by reflexivity.
+    rewrite<- sch_subst_instance; auto with kinding_regular.
+    apply type_equal_typ_subst with (J := K); assumption.
+  - apply typing_abs with (L := L \u \{X} \u dom E \u dom F).
     + replace knd_type with (knd_subst X S knd_type) by reflexivity.
       eauto using kinding_typ_subst.
     + fold (typ_subst X S T1).
@@ -126,7 +127,7 @@ Proof.
       rewrite <- env_subst_typ.
       auto using concat_assoc.
   - apply typing_let
-      with (L := L \u \{X} \u dom E0 \u dom F) (M := sch_subst X S M).
+      with (L := L \u \{X} \u dom E \u dom F) (M := sch_subst X S M).
     + introv Hf.
       autorewrite with rew_sch_arity in Hf.
       fresh_length Hf as Hl.
@@ -319,6 +320,188 @@ Proof.
   apply typing_typ_substs_l with (M := M); auto.
 Qed.
 
+(* Respects type equality *)
+
+Lemma typing_equal_binding : forall E F T1 T2 x t T,
+    type_equal E T1 T2 knd_type ->
+    typing (E & x ~: sch_empty T1 & F) t T ->
+    typing (E & x ~: sch_empty T2 & F) t T.
+Proof.
+  introv He Ht.
+  assert (valid_scheme E (sch_empty T2))
+    by (rewrite valid_scheme_empty_type;
+        auto with type_equal_validated).
+  apply validated_typing in Ht.
+  remember (E & x ~: sch_empty T1 & F) as ExF.
+  generalize dependent F.
+  induction Ht; intros; subst;
+    eauto using kinding_swap_typ_bind, subtype_swap_typ_bind.
+  - assert (valid_env (E & x ~: sch_empty T2 & F))
+      by eauto using valid_env_swap_typ_bind with typing_validated.
+    case_if_eq x x0.
+    + { assert (bind_typ M = bind_typ (sch_empty T1)) as Heq
+          by eauto using binds_middle_eq_inv, ok_from_environment.
+        assert
+          (valid_instance (E & x0 ~: sch_empty T1 & F) Us M) as Hi
+          by assumption.
+        inversion Heq; subst; inversion Hi; subst; simpl in *.
+        apply typing_var with (M := sch_empty T2) (Us := nil); auto.
+        - eauto using binds_middle_eq, ok_middle_inv_r,
+                      ok_from_environment, valid_instance_weakening,
+                      valid_instance_remove_typ_bind.
+        - eauto
+            using kinding_weakening_l, valid_env_retract
+            with type_equal_validated.
+        - apply type_equal_transitive with (T2 := T1);
+            eauto using type_equal_swap_typ_bind,
+                        type_equal_weakening_l, valid_env_retract. }
+    + apply typing_var with (M := M) (Us := Us);
+        eauto
+          using valid_instance_weakening,
+                valid_instance_remove_typ_bind,
+                type_equal_weakening, type_equal_remove_typ_bind,
+                binds_weakening, binds_subst
+          with valid_env_regular.
+  - econstructor;
+      eauto using kinding_swap_typ_bind.
+    introv Hn.
+    rewrite<- concat_assoc.
+    eauto using concat_assoc.
+  - econstructor.
+    + introv Hf.
+      rewrite<- concat_assoc.
+      eauto using concat_assoc.
+    + introv Hn.
+      rewrite<- concat_assoc.
+      eauto using concat_assoc.
+  - apply typing_match
+      with (L := L) (T1 := T0) (T2 := T3) (T3 := T4)
+           (T4 := T5) (T5 := T6) (T6 := T7) (T7 := T8);
+      eauto using kinding_swap_typ_bind, subtype_swap_typ_bind.
+    + introv Hn.
+      rewrite<- concat_assoc.
+      eauto using concat_assoc.
+    + introv Hn.
+      rewrite<- concat_assoc.
+      eauto using concat_assoc.
+  - econstructor;
+      eauto using kinding_swap_typ_bind, subtype_swap_typ_bind.
+    introv Hn.
+    rewrite<- concat_assoc.
+    eauto using concat_assoc.
+Qed.
+
+Lemma typing_equal_binding_l : forall E T1 T2 x t T,
+    type_equal E T1 T2 knd_type ->
+    typing (E & x ~: sch_empty T1) t T ->
+    typing (E & x ~: sch_empty T2) t T.
+Proof.
+  introv Hte Ht.
+  rewrite<- concat_empty_r with (E := E & x ~: sch_empty T2).
+  rewrite<- concat_empty_r with (E := E & x ~: sch_empty T1) in Ht.
+  eauto using typing_equal_binding.
+Qed.
+
+Lemma foo : forall E T1 T2 T3 T4 T5 T6,
+    kinding E T1 (knd_range T3 T4) ->
+    type_equal_cong E T1 T2 (knd_range T5 T6) ->
+    kinding E T2 (knd_range T3 T4).
+Proof.
+  introv Hk Hte.
+  remember (knd_range T5 T6) as K.
+  generalize dependent T5.
+  generalize dependent T6.
+  induction Hte; introv HeqK; inversion HeqK; subst.
+  - clear IHHte HeqK.
+    remember (typ_row T6) as T.
+    remember (knd_range T3 T4) as K.
+    generalize dependent T3.
+    generalize dependent T4.
+    induction Hk; introv HeqK; inversion HeqT; inversion HeqK;
+      subst; subst.
+    + apply kinding_range_subsumption
+        with (T1 := T1') (T2 := T1');
+        eauto using subtype_reflexive, type_equal_symmetric
+          with type_equal_cong_validated. 
+    + apply kinding_range_subsumption
+        with (T1 := T1) (T2 := T2); eauto.
+  - eauto.
+  - inversion H; subst.
+    + inversion H1.
+    + inversion H1.
+Qed.
+
+Lemma typing_equal_cong : forall E t T1 T2,
+    type_equal_cong E T1 T2 knd_type ->
+    typing E t T1 -> typing E t T2.
+Proof.
+  introv He Ht.
+  apply validated_typing in Ht.
+  generalize dependent T2.
+  induction Ht; introv He.
+  - apply typing_var with (M := M) (Us := Us); auto.
+    apply type_equal_transitive with (T2 := T);
+      eauto using type_equal_cong_symmetric.
+  - inversion He; subst.
+    + apply typing_abs with (L := L);
+        auto with type_equal_cong_validated.
+      introv Hn.
+      apply typing_equal_binding_l with (T1 := T1);
+        eauto with type_equal_cong_validated.
+    + apply typing_abs with (L := L \u dom E);
+        auto using type_equal_cong_weakening_l.
+    + { assert
+          (type_equal_symm E (typ_arrow T1 T2) T0 knd_type) as Hes
+          by assumption.
+        inversion Hes.
+        - assert
+            (type_equal_core E (typ_arrow T1 T2) T0 knd_type) as Hec
+            by assumption.
+          inversion Hec.
+        - assert
+            (type_equal_core E T0 (typ_arrow T1 T2) knd_type) as Hec
+            by assumption.
+          inversion Hec. }
+  - eauto.
+  - apply typing_let with (L := L \u dom E) (M := M);
+      auto using type_equal_cong_weakening_l.
+  - inversion He; subst.
+    + apply typing_constructor with (T2 := T2) (T3 := T3); auto.
+      eauto using foo.
+    + { assert
+          (type_equal_symm E (typ_variant T1) T0 knd_type) as Hes
+          by assumption.
+        inversion Hes.
+        - assert
+            (type_equal_core E (typ_variant T1) T0 knd_type) as Hec
+            by assumption.
+          inversion Hec.
+        - assert
+            (type_equal_core E T0 (typ_variant T1) knd_type) as Hec
+            by assumption.
+          inversion Hec. }
+  - apply typing_match
+      with (L := L) (T1 := T1) (T2 := T2) (T3 := T3)
+           (T4 := T4) (T5 := T5) (T6 := T6) (T7 := T7);
+      auto using type_equal_cong_weakening_l.
+  - apply typing_destruct
+      with (L := L) (T1 := T1) (T2 := T2) (T3 := T3);
+      auto using type_equal_cong_weakening_l.
+  - eauto with type_equal_cong_validated.
+Qed.
+
+Lemma typing_equal : forall E t T1 T2,
+    type_equal E T1 T2 knd_type ->
+    typing E t T1 -> typing E t T2.
+Proof.
+  introv Hte Ht.
+  remember knd_type as K.
+  induction Hte; subst;
+    eauto using typing_equal_cong.
+Qed.
+
+(* Term substitution *)
+
 Lemma typing_trm_subst : forall L E F x M s t T,
     typing (E & x ~: M & F) t T ->
     (forall Xs,
@@ -327,29 +510,66 @@ Lemma typing_trm_subst : forall L E F x M s t T,
     typing (E & F) (trm_subst x s t) T.
 Proof.
   introv Ht Hs.
+  assert (term s)
+    by (pick_freshes_gen L (sch_arity M) Ys;
+        specialize (Hs Ys Fr);
+        auto with typing_regular).
   remember (E & x ~: M & F) as ExF.
-  induction Ht; simpl.
+  apply validated_typing in Ht.
+  generalize dependent F.
+  induction Ht; intros; subst; simpl;
+    eauto using kinding_remove_typ_bind, subtype_remove_typ_bind.
   - case_var.
-    + subst.
-      assert (environment (E & x ~: M & F)) as He
-        by auto with valid_env_regular.
-      apply ok_from_environment in He.
-      assert (bind_typ M0 = bind_typ M) as Heq
-        by eauto using binds_middle_eq_inv.
+    + assert (bind_typ M0 = bind_typ M) as Heq
+        by eauto using binds_middle_eq_inv, ok_from_environment.
       inversion Heq; subst.
-      assert (valid_env (E & F))
-        by eauto using valid_env_typ_bind.
+      apply typing_equal with (T1 := instance M Us);
+        eauto using type_equal_symmetric, type_equal_remove_typ_bind.
       apply typing_instance with (L := L \u dom F);
-        eauto using valid_instance_typ_bind.
+        eauto using valid_instance_remove_typ_bind, valid_env_remove_typ_bind.
       introv Hf.
       assert (typing (E & Xs ~::* M) s (instance_vars M Xs)) as Ht
         by auto.
       assert (valid_env (E & Xs ~::* M))
         by auto with typing_validated.
       apply typing_weakening;
-        auto using valid_env_kinds_weakening_l.
-    + subst.
-      apply typing_var with (M := M0) (Us := Us);
-        eauto using valid_env_typ_bind, valid_instance_typ_bind.
+        eauto using valid_env_kinds_weakening_l, valid_env_remove_typ_bind.
+    + apply typing_var with (M := M0) (Us := Us);
+        eauto using valid_env_remove_typ_bind,
+          valid_instance_remove_typ_bind, type_equal_remove_typ_bind. 
       apply binds_subst with (x2 := x) (v2 := bind_typ M); auto.
-  - 
+  - apply typing_abs with (L := L0 \u \{x}).
+    + eauto using kinding_remove_typ_bind.
+    + introv Hn.
+      rewrite trm_subst_open_var; auto.
+      rewrite<- concat_assoc.
+      auto using concat_assoc.
+  - apply typing_let with (L := L0 \u \{x}) (M := M0).
+    + introv Hf.
+      rewrite<- concat_assoc.
+      auto using concat_assoc.
+    + introv Hn.
+      rewrite trm_subst_open_var; auto.
+      rewrite<- concat_assoc.
+      auto using concat_assoc.
+  - apply typing_match
+      with (L := L0 \u \{x}) (T1 := T1) (T2 := T2) (T3 := T3)
+           (T4 := T4) (T5 := T5) (T6 := T6) (T7 := T7);
+      eauto using kinding_remove_typ_bind, subtype_remove_typ_bind.
+    + introv Hn.
+      rewrite trm_subst_open_var; auto.
+      rewrite<- concat_assoc.
+      auto using concat_assoc.
+    + introv Hn.
+      rewrite trm_subst_open_var; auto.
+      rewrite<- concat_assoc.
+      auto using concat_assoc.
+  - apply typing_destruct
+      with (L := L0 \u \{x}) (T1 := T1) (T2 := T2) (T3 := T3);
+      eauto using kinding_remove_typ_bind, subtype_remove_typ_bind.
+    introv Hn.
+    rewrite trm_subst_open_var; auto.
+    rewrite<- concat_assoc.
+    auto using concat_assoc.
+Qed.
+
